finally done with SN

LeanScratch/Semantics/STLC/StrongNorm/ArgCount.lean
@@ -29,8 +29,8 @@ def Monotonic (v : ArgCount s) : Prop := match s with
   | .direct _ => True
   | .arr argTy _ =>
     -- Might need to add the restrictions Monotonic a and Monotonic b
-    (∀ a b : ArgCount argTy, lt a b → le (v a) (v b) ) ∧
-      (∀ x : ArgCount argTy, /- Monotonic x → -/ Monotonic (v x))
+    (∀ a b : ArgCount argTy, Monotonic a → Monotonic b →  le a b → le (v a) (v b)) ∧
+      (∀ x : ArgCount argTy, Monotonic x → Monotonic (v x))
 end
 
 instance : LT (ArgCount z) := ⟨lt⟩
@@ -103,9 +103,7 @@ theorem lt_trans {a b c : ArgCount t} (hab : a < b) (hbc : b < c) : a < c :=
     change lt _ _ at hab hbc ⊢
     simp only [lt] at hab hbc ⊢
     intro x xm
-    specialize hab x xm
-    specialize hbc x xm
-    exact lt_trans hab hbc
+    exact lt_trans (hab x xm) (hbc x xm)
 
 theorem le_trans {a b c : ArgCount t} (hab : a ≤ b) (hbc : b ≤ c) : a ≤ c :=
   match t with
@@ -131,7 +129,7 @@ theorem le_of_lt {a b : ArgCount z} : a < b → a ≤ b :=
   | .arr _ _ => by
     change lt _ _ → le _ _
     simp only [lt, le]
-    exact fun h x m => le_of_lt (h x m)
+    exact fun h x xm => le_of_lt (h x xm)
 
 theorem self_le_self {a : ArgCount z} : a ≤ a :=
   match z with
@@ -148,15 +146,21 @@ theorem zero_Monotonic : Monotonic (@zero s) := match s with
   | .direct _ => by simp only [Monotonic]
   | .arr _ _ => by
     simp only [Monotonic, zero]
-    exact ⟨fun _ _ _ => self_le_self, fun _ => zero_Monotonic⟩
+    exact ⟨fun _ _ _ _ _ => self_le_self, fun _ _ => zero_Monotonic⟩
 
 theorem le_congr
     {aF bF : ArgCount (.arr f r)}
     {aR bR : ArgCount f}
+    (hAFMono : Monotonic aF)
+    (hARMono : Monotonic aR)
+    (hBRMono : Monotonic bR)
     (hFLe : aF ≤ bF)
     (hRLe : aR ≤ bR)
-    : aF aR ≤ bF bR :=
-  sorry
+    : aF aR ≤ bF bR := by
+  change le _ _ at hFLe hRLe ⊢
+  simp only [le] at hFLe hRLe
+  simp only [Monotonic] at hAFMono hARMono
+  exact le_trans (hAFMono.1 aR bR hARMono hBRMono hRLe) (hFLe bR hBRMono)
 
 /- def strongNeq (a b : ArgCount z) : Prop := match z with -/
 /-   | .direct _ => a ≠ b -/
@@ -212,16 +216,28 @@ theorem lt_naturalize {a b : ArgCount v} (h : a < b) : naturalize a < naturalize
     simp only [ArgCount, lt, naturalize] at a b h ⊢
     exact lt_naturalize $ h zero zero_Monotonic
 
+theorem le_naturalize {a b : ArgCount v} (h : a ≤ b) : naturalize a ≤ naturalize b :=
+  match v with
+  | .direct _ => by
+    change le _ _ at h
+    simp only [le, naturalize] at h ⊢
+    exact h
+    /- h -/
+  | .arr _ _ => by
+    change le _ _ at h
+    simp only [ArgCount, le, naturalize] at a b h ⊢
+    exact le_naturalize $ h zero zero_Monotonic
+
 @[simp]
 theorem self_lt_addN {a : ArgCount t} (h : 0 < n) : a < addN a n :=
   match t with
   | .direct _ => by
     change lt _ _
-    simp only [ArgCount, addN, lt] at a ⊢
+    simp only [ArgCount, addN, le] at a ⊢
     exact Nat.lt_add_of_pos_right h
   | .arr _ _ => by
     change lt _ _
-    simp only [ArgCount, addN, lt] at a ⊢
+    simp only [ArgCount, addN, le] at a ⊢
     exact fun _ _ => self_lt_addN h
 
 @[simp]
@@ -235,7 +251,7 @@ theorem addN_lt_addN_right {a b : ArgCount t} (h : a < b) : addN a n < addN b n 
     change lt _ _ at h
     change lt _ _
     simp only [ArgCount, addN, lt] at a b h ⊢
-    exact fun z mz => addN_lt_addN_right (h z mz)
+    exact fun z zMono => addN_lt_addN_right (h z zMono)
 
 @[simp]
 theorem addN_lt_addN_left {n : ArgCount t} (h : a < b) : addN n a < addN n b := match t with
@@ -292,7 +308,7 @@ def addN_Monotonic {v : ArgCount s} (h : Monotonic v)
     simp only [addN, Monotonic] at h v ⊢
   | .arr _ _ => by
     simp only [addN, Monotonic] at h v ⊢
-    exact ⟨fun a b hLt => addN_le_addN_right (h.1 a b hLt), (addN_Monotonic $ h.right ·)⟩
+    exact ⟨fun a b aMono bMono hLt => addN_le_addN_right (h.1 a b aMono bMono hLt), (addN_Monotonic $ h.right · ·)⟩
 
 theorem le_addN_lt_lt {a b : ArgCount t} (hLe : a ≤ b) (hLt : n < m) : a.addN n < b.addN m :=
   match t with
@@ -306,6 +322,32 @@ theorem le_addN_lt_lt {a b : ArgCount t} (hLe : a ≤ b) (hLt : n < m) : a.addN 
     change lt _ _
     simp only [addN, lt, le] at hLe ⊢
     exact fun x xm => le_addN_lt_lt (hLe x xm) hLt
+
+theorem lt_sufficency
+    {a b : ArgCount (.arr f t)} {c : ArgCount f}
+    (cMono : Monotonic c)
+    (h : a < b) : a c < b c := by
+  change lt _ _ at h ⊢
+  simp only [lt] at *
+  exact h c cMono
+
+theorem le_trans_lt
+    {a b c : ArgCount t}
+    (h1 : a ≤ b)
+    (h2 : b < c)
+    : a < c :=
+  match t with
+  | .direct _ => by
+    change le _ _ at h1
+    change lt _ _ at h2 ⊢
+    simp only [le, lt, ArgCount] at a b c h1 h2 ⊢
+    exact Nat.lt_of_le_of_lt h1 h2
+  | .arr _ _ => by
+    change le _ _ at h1
+    change lt _ _ at h2 ⊢
+    simp only [le, lt, ArgCount] at a b c h1 h2 ⊢
+    intro x xm
+    exact le_trans_lt (h1 x xm) (h2 x xm)
 
 end ArgCount
 
